Update of Environments with a simpler definition of [length], more lemmas about [insert], etc.

Environments.v
@@ -129,6 +129,35 @@ Ltac one_plus_x_minus_one :=
 
 (* ---------------------------------------------------------------------------- *)
 
+(* Trivial facts. *)
+
+Lemma raw_insert_zero:
+  forall A o (e : env A),
+  raw_insert 0 o e = o :: e.
+Proof.
+  reflexivity.
+Qed.
+
+Lemma raw_insert_successor:
+  forall A x o (e : env A),
+  raw_insert (S x) o e =
+  lookup 0 e :: raw_insert x o (tail e).
+Proof.
+  intros. destruct e; reflexivity. (* ! *)
+Qed. (* Maybe this should be the definition of [raw_insert]. *)
+
+Lemma empty_eq_insert:
+  forall A x o (e : env A),
+  empty _ = insert x o e ->
+  False.
+Proof.
+  unfold empty; intros; destruct x.
+  rewrite raw_insert_zero in *. congruence.
+  rewrite raw_insert_successor in *. congruence.
+Qed.
+
+(* ---------------------------------------------------------------------------- *)
+
 (* Interaction between [lookup] and [empty]. *)
 
 Lemma lookup_empty_None:
@@ -144,6 +173,15 @@ Lemma lookup_empty_Some:
   False.
 Proof.
   destruct x; simpl; congruence.
+Qed.
+
+Lemma lookup_successor:
+  forall A x (e : env A),
+  lookup (S x) e = lookup x (tail e).
+Proof.
+  destruct e.
+  do 2 rewrite lookup_empty_None. reflexivity.
+  reflexivity.
 Qed.
 
 (* ---------------------------------------------------------------------------- *)
@@ -244,6 +282,15 @@ Qed.
 
 (* Interaction between [lookup] and [map]. *)
 
+Lemma lookup_map_none:
+  forall A B x e (f : A -> B),
+  lookup x e = None ->
+  lookup x (map f e) = None.
+Proof.
+  induction x; intros; destruct e as [ | [ | ] ? ]; simpl in *; subst;
+  solve [ eauto | congruence ].
+Qed.
+
 Lemma lookup_map_some:
   forall A B x a e (f : A -> B),
   lookup x e = Some a ->
@@ -253,6 +300,19 @@ Proof.
     congruence
   | eauto
   ].
+Qed.
+
+Lemma lookup_map_some_reverse:
+  forall A B x b e (f : A -> B),
+  lookup x (map f e) = Some b ->
+  exists a,
+  lookup x e = Some a /\ b = f a.
+Proof.
+  induction x; intros; destruct e as [ | [ | ] ? ]; simpl in *; subst; try solve [
+    congruence
+  | eauto
+  ].
+  eexists. split. reflexivity. congruence.
 Qed.
 
 (* ---------------------------------------------------------------------------- *)
@@ -275,6 +335,22 @@ Proof.
   destruct e; replace (1 + S s) with (S (1 + s)) by omega; simpl; f_equal; eauto with omega.
 Qed.
 
+(* Even when it is not known which of [k] and [s] is greater, [insert] commutes
+   with itself. The formula is slightly horrid, but can be very useful. *)
+
+Lemma insert_insert_always:
+  forall A k s (a b : option A) e,
+  raw_insert k a (raw_insert s b e) =
+  raw_insert (shift k s) b (raw_insert (if le_gt_dec k s then k else k - 1) a e).
+Proof.
+  intros.
+  destruct (le_gt_dec k s).
+  rewrite lift_idx_old by assumption. eauto using insert_insert.
+  rewrite lift_idx_recent by assumption.
+  replace k with (1 + (k - 1)) in * by omega. rewrite <- insert_insert by omega.
+  do 2 f_equal. omega.
+Qed.
+
 (* Attempting to rewrite in both directions may seem redundant, because of the
    symmetry of the law [insert_insert]. It is not: because [omega] fails in
    the presence of meta-variables, rewriting in one direction may be possible
@@ -294,6 +370,99 @@ Hint Extern 1 (_ = raw_insert _ _ (raw_insert _ _ _)) =>
   insert_insert
 : insert_insert.
 
+(* The result of an insertion cannot be nil. *)
+
+Lemma insert_nil:
+  forall A x a (e : env A),
+  insert x a e = nil ->
+  False.
+Proof.
+  destruct x; destruct e; simpl; congruence.
+Qed.
+
+(* Two lemmas about equations of the form [insert x a1 e1 = insert x a2 e2].
+   Note that we have [a1 = a2], but not [e1 = e2], due to padding. *)
+
+Lemma insert_eq_insert_1:
+  forall A x a1 a2 (e1 e2 : env A),
+  insert x a1 e1 = insert x a2 e2 ->
+  a1 = a2.
+Proof.
+  intros.
+  assert (lookup x (insert x a1 e1) = Some a1). eauto using lookup_insert_bingo.
+  assert (lookup x (insert x a2 e2) = Some a2). eauto using lookup_insert_bingo.
+  congruence.
+Qed.
+
+Lemma insert_eq_insert_2:
+  forall A x a1 a2 (e1 e2 : env A),
+  insert x a1 e1 = insert x a2 e2 ->
+  forall b,
+  insert x b e1 = insert x b e2.
+Proof.
+  induction x; simpl; intros.
+  congruence.
+  destruct e1; destruct e2;
+  match goal with h: _ = _ |- _ => injection h; clear h; intros end;
+  f_equal; try congruence; eauto.
+Qed.
+
+(* This is a really crazy diamond lemma that says, roughly, if the equation
+    [insert x1 a1 e1 = insert x2 a2 e2] holds, then [e1] and [e2] can be
+    constructed out of a common environment [e]. We would like to conclude
+    [e1 = insert x2 a2 e /\ e2 = insert x1 a1 e], but this is false, because
+    one of the indices is off-by-one in one way or the other. We need to
+    adjust, and the arithmetic is a bit painful. *)
+
+Lemma insert_eq_insert_3:
+  forall A x1 x2 a1 a2 (e1 e2 : env A),
+  insert x1 a1 e1 = insert x2 a2 e2 ->
+  x1 <> x2 ->
+  exists e y1 y2,
+  e1 = insert y1 a2 e /\
+  e2 = insert y2 a1 e /\
+  shift x1 y1 = x2 /\
+  y2 = (if le_gt_dec x1 y1 then x1 else x1 - 1).
+Proof.
+  induction x1; intros.
+  (* Case [x1 = 0]. *)
+  destruct x2; [ omega | ].
+  rewrite raw_insert_zero in *. rewrite raw_insert_successor in *.
+  match goal with h: _ = _ |- _ =>
+    injection h; clear h; intros
+  end.
+  destruct e2; [ congruence | ]. subst. simpl.
+  exists e2. exists x2. exists 0. eauto.
+  (* Case [x1 > 0]. *)
+  destruct x2.
+  (* Sub-case [x2 = 0]. *)
+  rewrite raw_insert_zero in *. rewrite raw_insert_successor in *.
+  match goal with h: _ = _ |- _ =>
+    injection h; clear h; intros
+  end.
+  destruct e1; [ congruence | ]. subst.
+  exists e1. exists 0. exists x1.
+  split. eauto.
+  split. eauto.
+  split. eauto.
+  dblib_by_cases. omega.
+  (* Sub-case [x2 > 0]. *)
+  do 2 rewrite raw_insert_successor in *.
+  assert (xx: x1 <> x2). omega.
+  match goal with h: _ = _ |- _ =>
+    injection h; clear h; intros h ?;
+    generalize (IHx1 _ _ _ _ _ h xx); intros [ e [ y1 [ y2 [ ? [ ? [ ? ? ]]]]]]
+  end.
+  (* [e1] and [e2] must be non-nil. *)
+  destruct e1; simpl tl in *; [ elimtype False; eauto using insert_nil | ].
+  destruct e2; simpl tl in *; [ elimtype False; eauto using insert_nil | ].
+  exists (o :: e). exists (S y1). exists (S y2).
+  split. simpl. congruence.
+  split. simpl. congruence.
+  split. eapply translate_lift with (k := 1). eauto.
+  dblib_by_cases; omega.
+Qed.
+
 (* ---------------------------------------------------------------------------- *)
 
 (* Interaction between [map] and [insert]. *)
@@ -305,6 +474,16 @@ Proof.
   induction x; intros; destruct e; simpl; eauto.
   rewrite IHx. reflexivity.
   match goal with o: option _ |- _ => destruct o end; f_equal; eauto.
+Qed.
+
+(* The following variant is easier to use for [eauto]. *)
+
+Lemma map_insert_eq:
+  forall A B (f : A -> B) x a b e,
+  f a = b ->
+  map f (insert x a e) = insert x b (map f e).
+Proof.
+  intros; subst. eapply map_insert.
 Qed.
 
 Ltac map_insert :=
@@ -364,6 +543,18 @@ Proof.
   eauto using map_map_exchange, @lift_lift.
 Qed.
 
+Lemma map_insert_map:
+  forall A (f g h : A -> A) x (a : A) e,
+  (forall a, f (g a) = g (h a)) ->
+  map f (insert x a (map g e)) =
+  insert x (f a) (map g (map h e)).
+Proof.
+  intros.
+  rewrite map_insert. f_equal.
+  eapply map_map_exchange.
+  eauto.
+Qed.
+
 Lemma map_map_vanish:
   forall A B (f : B -> A) (g : A -> B) (e : env A),
   (forall x, f (g x) = x) ->
@@ -417,26 +608,36 @@ Qed.
 
 (* ---------------------------------------------------------------------------- *)
 
-(* The definitions and properties that follow should be independent of the
-   details of the definitions of [empty], [lookup], [insert], and [map]. *)
+(* [length e] should be viewed as an upper bound on the true length of the
+   environment [e], since there may be useless [None] entries at the end.
+   We are careful to always work with hypotheses and goals of the form
+   [length e <= k]. *)
 
-Opaque empty lookup raw_insert map.
+Lemma length_monotonic:
+  forall A (e : env A) k1 k2,
+  length e <= k1 ->
+  k1 <= k2 ->
+  length e <= k2.
+Proof.
+  intros. omega.
+Qed.
 
-(* ---------------------------------------------------------------------------- *)
-
-(* A definition of (an upper bound on) the length of an environment. *)
-
-Definition length A (e : env A) (k : nat) :=
-  forall x,
-  k <= x ->
+Lemma lookup_beyond_length:
+  forall A (e : env A) x,
+  length e <= x ->
   lookup x e = None.
+Proof.
+  induction e; simpl; intros.
+  eapply lookup_empty_None.
+  destruct x; [ omega | ]. simpl. eapply IHe. omega.
+Qed.
 
 (* Every variable that is defined in the environment is less than the
    length of the environment. *)
 
 Lemma defined_implies_below_length:
   forall A (e : env A) x k a,
-  length e k ->
+  length e <= k ->
   lookup x e = Some a ->
   x < k.
 Proof.
@@ -445,7 +646,7 @@ Proof.
      [k <= x]. *)
   case (le_gt_dec k x); intro; try tauto.
   (* By definition of [length], [lookup x e] is [None]. *)
-  assert (lookup x e = None). auto.
+  assert (lookup x e = None). eapply lookup_beyond_length. omega.
   (* We obtain a contradiction. *)
   congruence.
 Qed.
@@ -456,24 +657,103 @@ Hint Resolve defined_implies_below_length : lift_idx_hints.
 
 Lemma length_empty:
   forall A k,
-  length (@empty A) k.
+  length (@empty A) <= k.
 Proof.
-  repeat intro. apply lookup_empty_None.
+  simpl. intros. omega.
 Qed.
 
-(* Extending an environment increments its length by one. *)
+(* This definition of [max] is much more pleasant to work with than the
+   one found in Coq's standard library. It can be easily unfolded, and
+   then [omega] takes control. *)
+
+Definition mymax m n :=
+  if le_gt_dec m n then n else m.
+
+Ltac mymax :=
+  unfold mymax in *; dblib_by_cases; try omega.
+
+(* Extending an environment increments its length by one, in the usual case.
+   It can be extended by more than one if [x] is far away. *)
+
+Lemma length_insert_general:
+  forall A x k o (e : env A),
+  length e = k ->
+  length (raw_insert x o e) = mymax (1 + k) (1 + x).
+Proof.
+  induction x; simpl; intros; subst.
+  mymax.
+  destruct e; simpl.
+  mymax. erewrite IHx by reflexivity. simpl. mymax.
+  erewrite IHx by reflexivity. mymax.
+Qed.
+
+(* This should be the usual case. *)
 
 Lemma length_insert:
-  forall A (e : env A) k o,
-  length e k ->
-  length (raw_insert 0 o e) (1 + k).
+  forall A x k km1 o (e : env A),
+  length e <= km1 ->
+  km1 <= k - 1 ->
+  x < k ->
+  length (raw_insert x o e) <= k.
 Proof.
-  unfold length; intros. lookup_insert. eauto with omega.
+  intros. erewrite length_insert_general by reflexivity. mymax.
 Qed.
 
-Hint Resolve length_empty length_insert : length.
+(* Pain, pain. *)
 
-Hint Resolve length_insert : construction_closed.
+Lemma length_insert_reverse_1:
+  forall A (e : env A) k x a,
+  length (insert x a e) <= k ->
+  x < k.
+Proof.
+  intros. erewrite length_insert_general in * by reflexivity. mymax.
+Qed.
+
+Lemma length_insert_reverse_2:
+  forall A (e : env A) k x a,
+  length (insert x a e) <= k + 1 ->
+  length e <= k.
+Proof.
+  intros. erewrite length_insert_general in * by reflexivity. mymax.
+Qed.
+
+Lemma length_insert_independent:
+  forall A (e : env A) k x a,
+  length (insert x a e) <= k ->
+  forall y o,
+  y < k ->
+  length (raw_insert y o e) <= k.
+Proof.
+  intros. erewrite length_insert_general in * by reflexivity. mymax.
+Qed.
+
+(* Applying a transformation to an environment does not affect its length. *)
+
+Lemma length_map_general:
+  forall A B (f : A -> B) (e : env A),
+  length (map f e) = length e.
+Proof.
+  induction e as [| [|] ]; simpl; intros; congruence.
+Qed.
+
+Lemma length_map:
+  forall A B (f : A -> B) (e : env A) k,
+  length e <= k ->
+  length (map f e) <= k.
+Proof.
+  intros. rewrite length_map_general. assumption.
+Qed.
+
+Hint Resolve length_empty length_insert length_map : length.
+
+Hint Resolve length_insert length_map : construction_closed.
+
+(* ---------------------------------------------------------------------------- *)
+
+(* The definitions and properties that follow should be independent of the
+   details of the definitions of [empty], [lookup], [insert], and [map]. *)
+
+Opaque empty lookup raw_insert map.
 
 (* ---------------------------------------------------------------------------- *)
 
@@ -489,20 +769,27 @@ Definition agree A (e1 e2 : env A) (k : nat) :=
 Lemma agree_below:
   forall A (e1 e2 : env A) x a k,
   lookup x e1 = Some a ->
-  length e1 k ->
+  x < k ->
   agree e1 e2 k ->
   lookup x e2 = Some a.
 Proof.
   do 6 intro. intros hlookup ? ?.
   rewrite <- hlookup. symmetry.
-  eauto using defined_implies_below_length.
+  eauto.
 Qed.
 
 (* The empty environment agrees with every environment up to length [0]. *)
 
-Lemma agree_empty:
+Lemma agree_empty_left:
   forall A (e : env A),
   agree (@empty _) e 0.
+Proof.
+  unfold agree. intros. elimtype False. omega.
+Qed.
+
+Lemma agree_empty_right:
+  forall A (e : env A),
+  agree e (@empty _) 0.
 Proof.
   unfold agree. intros. elimtype False. omega.
 Qed.
@@ -524,7 +811,226 @@ Proof.
   do 2 lookup_insert; eauto with omega.
 Qed.
 
-Hint Resolve agree_below agree_empty agree_insert : agree.
+Hint Resolve defined_implies_below_length agree_below agree_empty_left
+agree_empty_right agree_insert : agree.
+
+(* ---------------------------------------------------------------------------- *)
+
+(* A definition of when an environment subsumes another, up to a notion of
+   subsumption on environment entries. *)
+
+Section Subsume.
+
+  Variable A : Type.
+
+  Variable sub : A -> A -> Prop.
+
+  Variable sub_reflexive:
+    forall a,
+    sub a a.
+
+  Variable sub_transitive:
+    forall a1 a2 a3,
+    sub a1 a2 ->
+    sub a2 a3 ->
+    sub a1 a3.
+
+  (* Subsumption is first extended to options. *)
+
+  Definition osub (o1 o2 : option A) :=
+    forall a2,
+    o2 = Some a2 ->
+    exists a1,
+    o1 = Some a1 /\ sub a1 a2.
+
+  Lemma osub_None:
+    forall o,
+    osub o None.
+  Proof.
+    unfold osub. congruence.
+  Qed.
+
+  Lemma osub_Some_Some:
+    forall a1 a2,
+    sub a1 a2 ->
+    osub (Some a1) (Some a2).
+  Proof.
+    unfold osub. intros ? ? ? ? h. injection h; clear h; intro; subst; eauto.
+  Qed.
+
+  Lemma osub_None_Some:
+    forall a2,
+    osub None (Some a2) ->
+    False.
+  Proof.
+    unfold osub. intros ? h.
+    generalize (h _ eq_refl). clear h. intros [ a1 [ ? ? ]].
+    congruence.
+  Qed.
+
+  Lemma osub_Some_inversion:
+    forall o1 a2,
+    osub o1 (Some a2) ->
+    exists a1,
+    o1 = Some a1 /\ sub a1 a2.
+  Proof.
+    intros. destruct o1. eauto. elimtype False. eauto using osub_None_Some.
+  Qed.
+
+  (* Then, it is extended pointwise to environments. *)
+
+  Definition subsume (e1 e2 : env A) :=
+    forall x,
+    osub (lookup x e1) (lookup x e2).
+
+  (* Subsumption of environments is reflexive and transitive. *)
+
+  Lemma osub_reflexive:
+    forall o,
+    osub o o.
+  Proof.
+    unfold osub. eauto.
+  Qed.
+
+  Lemma subsume_reflexive:
+    forall e,
+    subsume e e.
+  Proof.
+    unfold subsume. eauto using osub_reflexive.
+  Qed.
+
+  Lemma osub_transitive:
+    forall o1 o2 o3,
+    osub o1 o2 ->
+    osub o2 o3 ->
+    osub o1 o3.
+  Proof.
+    unfold osub. intros ? ? ? hs1 hs2 a3 h3.
+    generalize (hs2 _ h3); intros [ a2 [ h2 ? ]].
+    generalize (hs1 _ h2); intros [ a1 [ h1 ? ]].
+    eauto.
+  Qed.
+
+  Lemma subsume_transitive:
+    forall e1 e2 e3,
+    subsume e1 e2 ->
+    subsume e2 e3 ->
+    subsume e1 e3.
+  Proof.
+    unfold subsume. eauto using osub_transitive.
+  Qed.
+
+  (* Every environment subsumes the empty environment. *)
+
+  Lemma subsume_empty:
+    forall e,
+    subsume e (@empty _).
+  Proof.
+    unfold subsume. intros. rewrite lookup_empty_None. apply osub_None.
+  Qed.
+
+  (* Extending two environments with a new variable preserves subsumption. *)
+
+  Lemma subsume_insert:
+    forall e1 e2,
+    subsume e1 e2 ->
+    forall x o1 o2,
+    osub o1 o2 ->
+    subsume (raw_insert x o1 e1) (raw_insert x o2 e2).
+  Proof.
+    unfold subsume. do 7 intro. intros n.
+    (* Reason by cases: [x = n], [x < n], [x > n]. *)
+    case (le_gt_dec x n); [ case (eq_nat_dec x n) | ]; intros;
+    (* In each case, [lookup_insert] simplifies the goal. *)
+    repeat lookup_insert; eauto.
+  Qed.
+
+  Lemma subsume_cons:
+    forall o e1 e2,
+    osub o (lookup 0 e2) ->
+    subsume e1 (tl e2) ->
+    subsume (o :: e1) e2.
+  Proof.
+    do 3 intro. intros h1 h2. intro n. destruct n.
+    eauto.
+    do 2 rewrite lookup_successor. eauto.
+  Qed.
+
+  Lemma subsume_cons_cons_inversion:
+    forall o1 o2 e1 e2,
+    subsume (o1 :: e1) (o2 :: e2) ->
+    osub o1 o2 /\
+    subsume e1 e2.
+  Proof.
+    do 4 intro. intro h.
+    split.
+    eapply (h 0).
+    intro n. eapply (h (1 + n)).
+  Qed.
+
+  Lemma subsume_insert_inversion:
+    forall e1 x a2 e2,
+    subsume e1 (insert x a2 e2) ->
+    exists f1 a1,
+    e1 = insert x a1 f1 /\
+    subsume f1 e2 /\
+    sub a1 a2.
+  Proof.
+    (* Really painful. *)
+    induction e1; simpl; intros.
+    (* Base. *)
+    elimtype False.
+    match goal with h: subsume nil _ |- _ =>
+      generalize (h x); clear h; intro h;
+      rewrite lookup_insert_bingo in h by reflexivity;
+      rewrite lookup_empty_None in h
+    end.
+    solve [ eauto using osub_None_Some ].
+    (* Step. *)
+    destruct x.
+    (* Case [x = 0]. *)
+    match goal with h: subsume _ _ |- _ =>
+      rewrite raw_insert_zero in h;
+      generalize (subsume_cons_cons_inversion h); clear h; intros [ h ? ];
+      generalize (osub_Some_inversion h); intros [ ? [ ? ? ]]; subst
+    end.
+    do 2 eexists.
+    rewrite raw_insert_zero.
+    solve [ eauto ].
+    (* Case [x > 0]. *)
+    match goal with h: subsume _ _ |- _ =>
+      rewrite raw_insert_successor in h;
+      generalize (subsume_cons_cons_inversion h); clear h; intros [ ? h ];
+      generalize (IHe1 _ _ _ h); clear IHe1; intros [ f1 [ a1 [ ? [ ? ? ]]]]; subst
+    end.
+    exists (a :: f1). exists a1.
+    rewrite raw_insert_successor. simpl.
+    split; [ | split ].
+    reflexivity.
+    eauto using subsume_cons.
+    eauto.
+  Qed.
+
+  (* Applying a transformation [f] pointwise to two environments preserves
+     environment subsumption, provided [f] preserves [sub]. *)
+
+  Lemma subsume_map:
+    forall f,
+    (forall a1 a2, sub a1 a2 -> sub (f a1) (f a2)) ->
+    forall e1 e2,
+    subsume e1 e2 ->
+    subsume (map f e1) (map f e2).
+  Proof.
+    intros ? hf ? ? hs. intros ? b2 hlm2.
+    generalize (lookup_map_some_reverse _ _ _ hlm2); intros [ ? [ hl2 ? ]]. subst.
+    generalize (hs _ _ hl2); intros [ a1 [ ? ? ]].
+    eauto using lookup_map_some.
+  Qed.
+
+End Subsume.
+
+Hint Resolve osub_reflexive osub_Some_Some subsume_reflexive
+subsume_transitive subsume_empty subsume_insert subsume_map : subsume.
 
 (* ---------------------------------------------------------------------------- *)
 
@@ -547,15 +1053,22 @@ Fixpoint concat (A : Type) (e1 : env A) (e2 : list A) : env A :=
 (* Concatenation acts upon the length of the environment in an obvious
    manner. *)
 
+Lemma omega_hint_1:
+  forall n,
+  n <= (n + 1) - 1.
+Proof.
+  intros. omega.
+Qed.
+
 Lemma length_concat:
   forall A (e2 : list A) (e1 : env A) n1 n,
-  length e1 n1 ->
-  n1 + List.length e2 = n ->
-  length (concat e1 e2) n.
+  length e1 <= n1 ->
+  n1 + length e2 = n ->
+  length (concat e1 e2) <= n.
 Proof.
   induction e2; simpl; intros.
   replace n with n1 by omega. assumption.
-  eauto using length_insert with omega.
+  eauto using length_insert, omega_hint_1 with omega.
 Qed.
 
 Hint Resolve length_concat : length construction_closed.
@@ -566,7 +1079,7 @@ Hint Resolve length_concat : length construction_closed.
 Lemma agree_concat:
   forall A (e : list A) (e1 e2 : env A) k n,
   agree e1 e2 k ->
-  k + List.length e = n ->
+  k + length e = n ->
   agree (concat e1 e) (concat e2 e) n.
 Proof.
   induction e; simpl; intros.
@@ -580,7 +1093,7 @@ Hint Resolve agree_concat : agree.
 
 Lemma insert_concat:
   forall (A : Type) n x nx (o : option A) e1 e2,
-  List.length e2 = n ->
+  length e2 = n ->
   n + x = nx ->
   raw_insert nx o (concat e1 e2) = concat (raw_insert x o e1) e2.
 Proof.
@@ -605,7 +1118,7 @@ Fixpoint replicate (A : Type) (n : nat) (a : A) : list A :=
 
 Lemma length_replicate:
   forall (A : Type) n (a : A),
-  List.length (replicate n a) = n.
+  length (replicate n a) = n.
 Proof.
   induction n; simpl; auto.
 Qed.
@@ -637,9 +1150,9 @@ concat_replicate_is_iterated_insert : insert_concat.
 
 Lemma length_concat_replicate:
   forall A (a : A) (e1 : env A) n1 n2 n,
-  length e1 n1 ->
+  length e1 <= n1 ->
   n1 + n2 = n ->
-  length (concat e1 (replicate n2 a)) n.
+  length (concat e1 (replicate n2 a)) <= n.
 Proof.
   intros. eapply length_concat. eauto. rewrite length_replicate. eauto.
 Qed.
